Add Umap_Uctor goal to model axioms

Composition.thy
@@ -48,19 +48,6 @@ ML \<open>
 val tau = the (MRBNF_Def.mrbnf_of @{context} "Composition.\<tau>_pre")
 \<close>
 
-lemma image_in_bij_eq: "bij f \<Longrightarrow> (a \<in> f ` A) = (inv f a \<in> A)"
-  by force
-
-lemma supp_comp_bound:
-  assumes bound: "|supp f| <o |UNIV::'a set|" "|supp g| <o |UNIV::'a set|"
-  and inf: "infinite (UNIV::'a set)"
-  shows "|supp (g \<circ> f)| <o |UNIV::'a set|"
-proof -
-  from inf bound(2,1) have "|supp g \<union> supp f| <o |UNIV::'a set|" by (rule card_of_Un_ordLess_infinite)
-  then show ?thesis using supp_o
-    by (metis card_of_mono1 ordLeq_ordLess_trans)
-qed
-
 ML_file \<open>Tools/mrbnf_fp_tactics.ML\<close>
 ML_file \<open>Tools/mrbnf_fp.ML\<close>
 
@@ -80,63 +67,162 @@ end
 print_theorems
 term "\<tau>_ctor"
 
-ML_file \<open>Tools/mrbnf_recursor.ML\<close>
+lemma infinite_var_\<tau>_pre: "infinite (UNIV :: 'a::var_\<tau>_pre set)"
+  using card_of_ordLeq_finite cinfinite_def infinite_regular_card_order.Cinfinite infinite_regular_card_order_card_suc natLeq_Card_order natLeq_card_order natLeq_cinfinite var_DEADID_class.large by blast
 
-definition FFVars_\<tau>' :: "'a::var_\<tau>_pre \<tau> \<Rightarrow> 'a \<tau> \<Rightarrow> 'a set"
-  where "FFVars_\<tau>' \<equiv> undefined"
-definition rrename_\<tau>' :: "('a \<Rightarrow> 'a) \<Rightarrow> 'a::var_\<tau>_pre \<tau> \<Rightarrow> 'a \<tau> \<Rightarrow> 'a \<tau>"
-  where "rrename_\<tau>' \<equiv> undefined"
+(******************** Definitions for variable-for-variable substitution ***********)
+typedef 'a :: var_\<tau>_pre ssfun = "{f :: 'a \<Rightarrow> 'a. |supp f| <o |UNIV::'a set|}"
+  by (auto intro!: exI[of _ id] simp: supp_id_bound)
+
+setup_lifting type_definition_ssfun
+
+lift_definition idSS :: "'a ::var_\<tau>_pre ssfun" is id
+  by (simp add: supp_id_bound)
+
+lemma supp_comp_bound_var_\<tau>_pre: "\<lbrakk> |supp f| <o |UNIV::'a::var_\<tau>_pre set| ; |supp g| <o |UNIV::'a set| \<rbrakk> \<Longrightarrow> |supp (g \<circ> f)| <o |UNIV::'a set|"
+  using infinite_var_\<tau>_pre supp_comp_bound by blast
+
+context
+  fixes u :: "'a :: var_\<tau>_pre \<Rightarrow> 'a"
+  assumes u: "bij u" "|supp u| <o |UNIV::'a set|"
+begin
+  lift_definition compSS :: "'a ::var_\<tau>_pre ssfun \<Rightarrow> 'a ssfun" is "\<lambda>p. u o p o inv u"
+    by (simp add: supp_comp_bound_var_\<tau>_pre supp_inv_bound u)
+end
+
+lemma compSS_id: "compSS id = id"
+  supply supp_id_bound[transfer_rule] bij_id[transfer_rule] by (rule ext, transfer) auto
+lemma compSS_comp:
+  fixes f :: "'a::var_\<tau>_pre \<Rightarrow> 'a" and g :: "'a \<Rightarrow> 'a"
+  assumes "bij f" "|supp f| <o |UNIV::'a set|" "bij g" "|supp g| <o |UNIV::'a set|"
+  shows "compSS (f \<circ> g) = compSS f \<circ> compSS g"
+  supply assms[transfer_rule] bij_comp[transfer_rule] supp_comp_bound_var_\<tau>_pre[transfer_rule]
+  by (rule ext, transfer) (auto simp: fun_eq_iff assms o_inv_distrib)
+lemma compSS_cong_id:
+  fixes f :: "'a::var_\<tau>_pre \<Rightarrow> 'a" and d :: "'a ssfun"
+  assumes "bij f" "|supp f| <o |UNIV|" "\<And>a. a \<in> imsupp (Rep_ssfun d) \<Longrightarrow> f a = a"
+  shows "compSS f d = d"
+  supply assms(1,2)[transfer_rule]
+  using assms(3)
+  apply (transfer fixing: f)
+  oops
+
+lemma imsupp_ssfun_bound:
+  fixes p :: "'a::var_\<tau>_pre ssfun"
+  shows "|imsupp (Rep_ssfun p)| <o |UNIV::'a set|"
+  unfolding imsupp_def
+  apply (rule card_of_Un_ordLess_infinite)
+    apply (rule infinite_var_\<tau>_pre)
+  using Rep_ssfun apply blast
+  by (metis Rep_ssfun card_of_image mem_Collect_eq ordLeq_ordLess_trans)
+
+definition CCTOR' :: "('a::var_\<tau>_pre, 'a, 'a ssfun \<Rightarrow> 'a \<tau>, 'a ssfun \<Rightarrow> 'a \<tau>) \<tau>_pre \<Rightarrow> 'a ssfun \<Rightarrow> 'a \<tau>" where
+  "CCTOR' \<equiv> \<lambda>F p. \<tau>_ctor (map_\<tau>_pre (Rep_ssfun p) id (\<lambda>R. R p) (\<lambda>R. R p) F)"
+definition CCTOR :: "('a::var_\<tau>_pre, 'a, 'a \<tau> \<times> ('a ssfun \<Rightarrow> 'a \<tau>), 'a \<tau> \<times> ('a ssfun \<Rightarrow> 'a \<tau>)) \<tau>_pre \<Rightarrow> 'a ssfun \<Rightarrow> 'a \<tau>" where
+  "CCTOR = (\<lambda>F p. \<tau>_ctor (map_\<tau>_pre (Rep_ssfun p) id ((\<lambda>R. R p) o snd) ((\<lambda>R. R p) o snd) F))"
+(*definition Umap :: "('a::var_\<tau>_pre \<Rightarrow> 'a) \<Rightarrow> 'a \<tau> \<Rightarrow> ('a ssfun \<Rightarrow> 'a \<tau>) \<Rightarrow> ('a ssfun \<Rightarrow> 'a \<tau>)" where
+  "Umap f t pu \<equiv> \<lambda>c. rrename_\<tau> f (pu (compSS (inv f) c))"*)
+definition Umap :: "('a::var_\<tau>_pre \<Rightarrow> 'a) \<Rightarrow> 'a \<tau> \<Rightarrow> 'a \<tau> \<Rightarrow> 'a \<tau>" where
+  "Umap f t \<equiv> rrename_\<tau> f"
+definition UFVars :: "'a::var_\<tau>_pre \<tau> \<Rightarrow> 'a \<tau> \<Rightarrow> 'a set" where
+  "UFVars t \<equiv> FFVars_\<tau>"
+lemma Umap_id0: "Umap id t = id"
+  unfolding Umap_def
+  by (rule \<tau>.rrename_id0s)
+lemma Umap_cong_id:
+  fixes f :: "'a::var_\<tau>_pre \<Rightarrow> 'a"
+  assumes "bij f" "|supp f| <o |UNIV::'a set|" "\<And>z. z \<in> UFVars t w \<Longrightarrow> f z = z"
+  shows "Umap f t w = w"
+  using assms unfolding Umap_def UFVars_def
+  by (rule \<tau>.rrename_cong_ids)
+
+(***************************************************************************************)
+
+
+
+
+
+
+
+
+
+
+
+
+
+
+
+ML_file \<open>Tools/mrbnf_recursor.ML\<close>
 
 local_setup \<open>fn lthy =>
 let
+  fun rtac ctxt = resolve_tac ctxt o single
+  val model_ext_tacs = {
+    small_avoiding_sets = [fn ctxt => rtac ctxt @{thm emp_bound} 1],
+    Umap_id0 = fn ctxt => resolve_tac ctxt @{thms Umap_id0} 1,
+    Umap_comp0 = fn ctxt => Skip_Proof.cheat_tac ctxt 1,
+    Umap_cong_ids = map (fn thm => fn ctxt => EVERY1 [
+      resolve_tac ctxt [thm],
+      REPEAT_DETERM o (Goal.assume_rule_tac ctxt ORELSE' assume_tac ctxt)
+    ]) @{thms Umap_cong_id},
+    in_UFVars_Umap = [fn ctxt => Skip_Proof.cheat_tac ctxt 1],
+    Umap_Uctor = fn ctxt => Skip_Proof.cheat_tac ctxt 1
+  };
   val model_tacs = {
+    small_avoiding_sets = [fn ctxt => rtac ctxt @{thm emp_bound} 1],
     Umap_id0 = fn ctxt => resolve_tac ctxt @{thms \<tau>.rrename_id0s} 1,
     Umap_comp0 = fn ctxt => Skip_Proof.cheat_tac ctxt 1,
     Umap_cong_ids = map (fn thm => fn ctxt => EVERY1 [
       resolve_tac ctxt [thm],
       REPEAT_DETERM o (Goal.assume_rule_tac ctxt ORELSE' assume_tac ctxt)
     ]) @{thms \<tau>.rrename_cong_ids},
-    in_UFVars_Umap = [fn ctxt => Skip_Proof.cheat_tac ctxt 1]
+    in_UFVars_Umap = [fn ctxt => Skip_Proof.cheat_tac ctxt 1],
+    Umap_Uctor = fn ctxt => Skip_Proof.cheat_tac ctxt 1
   };
   val parameter_tacs = {
-    Pmap_id0 = fn ctxt => Skip_Proof.cheat_tac ctxt 1,
-    Pmap_comp0 = fn ctxt => Skip_Proof.cheat_tac ctxt 1,
+    Pmap_id0 = fn ctxt => rtac ctxt @{thm compSS_id} 1,
+    Pmap_comp0 = fn ctxt => EVERY1 [rtac ctxt @{thm compSS_comp}, REPEAT_DETERM o assume_tac ctxt],
     Pmap_cong_ids = [fn ctxt => Skip_Proof.cheat_tac ctxt 1],
     in_PFVars_Pmap = [fn ctxt => Skip_Proof.cheat_tac ctxt 1],
-    small_PFVars = [fn ctxt => Skip_Proof.cheat_tac ctxt 1]
+    small_PFVars = [fn ctxt => rtac ctxt @{thm imsupp_ssfun_bound} 1]
   };
   val model_ext = {
     U = @{typ "'a::var_\<tau>_pre \<tau>"},
     term_quotient = SOME {
       qT = @{typ "'a::var_\<tau>_pre \<tau>"},
-      qmap = @{term rrename_\<tau>}
+      qmap = @{term rrename_\<tau>},
+      qctor = @{term \<tau>_ctor}
     },
-    UFVars = [@{term "FFVars_\<tau>'"}],
-    Umap = @{term "rrename_\<tau>'"},
-    Uctor = @{term \<tau>_ctor},
+    UFVars = [@{term "UFVars"}],
+    Umap = @{term "Umap"},
+    Uctor = @{term CCTOR},
+    avoiding_sets = [@{term "{} :: 'a::var_\<tau>_pre set"}],
+    mrbnf = tau,
     parameters = {
-      P = @{typ "unit"},
-      PFVars = [@{term "\<lambda>_. {}"}],
-      Pmap = @{term "id :: ('a => 'a) => 'a => 'a"},
+      P = @{typ "'a::var_\<tau>_pre ssfun"},
+      PFVars = [@{term "\<lambda>p. imsupp (Rep_ssfun p)"}],
+      Pmap = @{term "compSS"},
       axioms = parameter_tacs
     },
-    axioms = model_tacs
+    axioms = model_ext_tacs
   };
   val model = {
     U = @{typ "'a::var_\<tau>_pre \<tau>"},
     term_quotient = NONE,
     UFVars = [@{term "FFVars_\<tau>"}],
     Umap = @{term "rrename_\<tau>"},
-    Uctor = @{term \<tau>_ctor},
+    Uctor = @{term CCTOR'},
+    avoiding_sets = [@{term "{} :: 'a::var_\<tau>_pre set"}],
+    mrbnf = tau,
     parameters = {
-      P = @{typ "unit"},
-      PFVars = [@{term "\<lambda>_. {}"}],
-      Pmap = @{term "id :: ('a => 'a) => 'a => 'a"},
+      P = @{typ "'a::var_\<tau>_pre ssfun"},
+      PFVars = [@{term "\<lambda>p. imsupp (Rep_ssfun p)"}],
+      Pmap = @{term "compSS"},
       axioms = parameter_tacs
     },
     axioms = model_tacs
   };
-  val lthy' = MRBNF_Recursor.create_binding_recursor model lthy
+  val lthy' = MRBNF_Recursor.create_binding_recursor model_ext lthy
 in lthy' end
 \<close>
 
